Update.

src/metalogic/hol.lean
@@ -34,3 +34,37 @@ def model.type (M : model) (V : valuation) : hol_type → Type
 | (var α) := V α
 | (const n ν args) := M n ν (fun i : fin n, model.type (args i))
 | (func σ₁ σ₂) := model.type σ₁ → model.type σ₂
+
+def hol_type.instance (type_var_symbol_to_type : type_var_symbols → hol_type) : hol_type → hol_type
+| (var α) := type_var_symbol_to_type α
+| (const n ν args) := const n ν (fun i : fin n, hol_type.instance (args i))
+| (func σ₁ σ₂) := func (hol_type.instance σ₁) (hol_type.instance σ₂)
+
+lemma lem_1
+	(σ : hol_type)
+	(m₁ m₂ : type_var_symbols → hol_type)
+	(h1 : σ.instance m₁ = σ.instance m₂) :
+	∀ α ∈ σ.var_set, m₁ α = m₂ α :=
+begin
+	intros α' h2,
+	induction σ,
+	case hol_type.var : α
+  {
+		unfold hol_type.instance at h1, unfold hol_type.var_set at h2,
+		simp only [finset.mem_singleton] at h2, subst h2, exact h1,
+	},
+  case hol_type.const : n ν args σ_ih
+  { unfold hol_type.instance at h1, unfold hol_type.var_set at h2,
+		simp at h1,
+		simp at h2, apply exists.elim h2, intros i h3,
+		apply σ_ih i, sorry, exact h3,
+},
+  case hol_type.func : σ₁ σ₂ σ₁_ih σ₂_ih
+  {
+		unfold hol_type.instance at h1, unfold hol_type.var_set at h2,
+		simp at h1, cases h1,
+		simp at h2, cases h2,
+		exact σ₁_ih h1_left h2,
+		exact σ₂_ih h1_right h2,
+	},
+end
